gate generic call summaries to closed type args

fixtures/TypeChecker.ml
@@ -12941,6 +12941,11 @@ let supported_type_generic_function_value_call_callee_ty_b t =
      | _ -> false)
   | _ -> false
 
+(** val type_args_lbound_free_b : ty list -> bool **)
+
+let type_args_lbound_free_b type_args =
+  forallb (fun t -> negb (contains_lbound_ty t)) type_args
+
 (** val check_supported_non_type_generic_function_value_call_expr :
     global_env -> outlives_ctx -> Big_int_Z.big_int -> root_env -> ctx ->
     expr -> bool **)
@@ -12958,18 +12963,21 @@ let check_supported_non_type_generic_function_value_call_expr env _UU03a9_ n r _
 
 (** val check_supported_type_generic_function_value_call_expr :
     global_env -> outlives_ctx -> Big_int_Z.big_int -> root_env -> ctx ->
-    expr -> bool **)
+    expr -> ty list -> bool **)
 
-let check_supported_type_generic_function_value_call_expr env _UU03a9_ n r _UU0393_ callee = match callee with
-| EVar _ ->
-  (match infer_core_env_roots_shadow_safe env _UU03a9_ n r _UU0393_ callee with
-   | Infer_ok p ->
-     let (p0, _) = p in
-     let (p1, _) = p0 in
-     let (t_callee, _) = p1 in
-     supported_type_generic_function_value_call_callee_ty_b t_callee
-   | Infer_err _ -> false)
-| _ -> false
+let check_supported_type_generic_function_value_call_expr env _UU03a9_ n r _UU0393_ callee type_args =
+  (&&) (type_args_lbound_free_b type_args)
+    (match callee with
+     | EVar _ ->
+       (match infer_core_env_roots_shadow_safe env _UU03a9_ n r _UU0393_
+                callee with
+        | Infer_ok p ->
+          let (p0, _) = p in
+          let (p1, _) = p0 in
+          let (t_callee, _) = p1 in
+          supported_type_generic_function_value_call_callee_ty_b t_callee
+        | Infer_err _ -> false)
+     | _ -> false)
 
 (** val check_fn_root_shadow_non_capturing_call_provenance_summary :
     global_env -> fn_def -> bool **)
@@ -13391,10 +13399,10 @@ let rec check_expr_root_shadow_store_safe_narrow_summary_fuel fuel env _UU03a9_ 
          (&&) (store_safe_function_value_call_args_b env args)
            (check_supported_non_type_generic_function_value_call_expr env
              _UU03a9_ n r (ctx_of_sctx _UU03a3_) callee)
-       | ECallExprGeneric (callee, _, args) ->
+       | ECallExprGeneric (callee, type_args, args) ->
          (&&) (store_safe_function_value_call_args_b env args)
            (check_supported_type_generic_function_value_call_expr env
-             _UU03a9_ n r (ctx_of_sctx _UU03a3_) callee)
+             _UU03a9_ n r (ctx_of_sctx _UU03a3_) callee type_args)
        | EStruct (name, _, _, l1) ->
          (match l1 with
           | [] ->
